\documentclass[12pt]{article}
 
\usepackage[margin=1in]{geometry} 
\usepackage{amsmath,amsthm,amssymb}
\usepackage{listings}
\usepackage{tikz}
\usepackage{colortbl}
\usepackage{verbatim}
\usetikzlibrary{arrows, angles, quotes}
\usepackage{framed}
\usepackage{indentfirst}

\lstset{basicstyle=\footnotesize}
\usetikzlibrary{calc}

 
\newenvironment{theorem}[2][Theorem]{\begin{trivlist}
\item[\hskip \labelsep {\bfseries #1}\hskip \labelsep {\bfseries #2.}]}{\end{trivlist}}
\newenvironment{lemma}[2][Lemma]{\begin{trivlist}
\item[\hskip \labelsep {\bfseries #1}\hskip \labelsep {\bfseries #2.}]}{\end{trivlist}}
\newenvironment{exercise}[2][Exercise]{\begin{trivlist}
\item[\hskip \labelsep {\bfseries #1}\hskip \labelsep {\bfseries #2.}]}{\end{trivlist}}
\newenvironment{problem}[2][Problem]{\begin{trivlist}
\item[\hskip \labelsep {\bfseries #1}\hskip \labelsep {\bfseries #2.}]}{\end{trivlist}}
\newenvironment{question}[2][Question]{\begin{trivlist}
\item[\hskip \labelsep {\bfseries #1}\hskip \labelsep {\bfseries #2.}]}{\end{trivlist}}
\newenvironment{corollary}[2][Corollary]{\begin{trivlist}
\item[\hskip \labelsep {\bfseries #1}\hskip \labelsep {\bfseries #2.}]}{\end{trivlist}}

\newenvironment{solution}{\begin{proof}[Solution]}{\end{proof}}
 
\begin{document}
 
\title{Homework 4\\
    \large CS128 Intro to Higher Mathematics}
\author{Harry Coleman}
\date{October 10, 2019}

\maketitle

\section*{Exercise 3}
\begin{framed}
    Give a deduction of $p$ from the set $\{((\neg s) \lor r), (r \rightarrow p), s\}.$
\end{framed}

\begin{center}
    \begin{tabular}{r l l}
        1 & $\lnot s \lor r$ & Hypothesis \\
        2 & $r \implies p$ & Hypothesis \\
        3 & $s$ & Hypothesis \\
        \hline
        4 & $s \implies r$ & Definition of Implication on line 1 \\
        5 & $s \implies p$ & Transitivity on lines 2, 4 \\
        \hline
        6 & p & Modus Ponens on lines 3, 5
    \end{tabular}    
\end{center}

\newpage
\section*{Exercise 4}
\begin{framed}
    Show that the conclusion follows from the premises of the following formal argument using a deduction.

    \begin{enumerate}
    \item $u \lor r$
    \item $(r \rightarrow (\neg q)) \land t$
    \item $(s \lor w) \rightarrow (\neg p)$
    \item $u\rightarrow w$
    \end{enumerate}
    Conclusion: $(\neg p) \lor (\neg q)$.
\end{framed}


\begin{center}
    \begin{tabular}{r l l}
        1 & $u \lor r$ & Hypothesis \\
        2 & $(r \rightarrow (\neg q)) \land t$ & Hypothesis \\
        3 & $(s \lor w) \rightarrow (\neg p)$ & Hypothesis \\
        4 & $u\rightarrow w$ & Hypotheis \\
        \hline
        5 & $\lnot(s \lor w) \lor (\lnot p)$ & Definition of Implication on line 3 \\
        6 & $(\lnot s \land \lnot w) \lor (\lnot p)$ & De Morgan's Laws on line 5 \\
        7 & $(\lnot p \lor \lnot s) \land (\lnot p \lor \lnot w)$ & Distribution on line 6 \\
        8 & $\lnot p \lor \lnot w$ & Simplification on line 7 \\
        9 & $p \implies \lnot w$ & Definition of Implication on line 8 \\
        10 & $\lnot w \implies \lnot u$ & Contrapositive on line 4 \\
        11 & $p \implies \lnot u$ & Transitivity on lines 9, 10 \\
        12 & $\lnot u \implies r$ & Definition of Implication on line 1 \\
        13 & $p \implies r$ & Transitivity on lines 11, 12 \\
        14 & $r \implies \lnot q$ & Simplification on line 2 \\
        15 & $p \implies \lnot q$ & Transitivity on lines 13, 14 \\
        \hline
        16 & $\lnot p \lor \lnot q$ & Definition of Implication on line 15
    \end{tabular}    
\end{center}


\newpage
\section*{Exercise 6}
\begin{framed}
    Show that 
    \[((\sigma_1 \land \cdots \land \sigma_k) \rightarrow \tau) \equiv (\sigma_1 \rightarrow ( \sigma_2  \rightarrow (\cdots  \rightarrow (\sigma_k \rightarrow \tau)))).\]
\end{framed}

\begin{center}
    \begin{tabular}{r l l}
        $((\sigma_1 \land \cdots \land \sigma_k) \rightarrow \tau)$ & $\equiv (\lnot (\sigma_1 \land \cdots \land \sigma_k) \lor \tau)$ & Definition of Implication \\
        &$\equiv ((\lnot \sigma_1 \lor \cdots \lor \lnot \sigma_k) \lor \tau)$ & De Morgan's Laws \\
        &$\equiv (\lnot \sigma_1 \lor (\lnot \sigma_2 \lor ( \cdots (\lnot \sigma_k \lor \tau))))$ & Associativity of Disjunction \\
        &$\equiv (\sigma_1 \implies (\sigma_2 \implies ( \cdots (\sigma_k \implies \tau))))$ & Definition of Implication 
        
    \end{tabular}
\end{center}

Therefore
\[((\sigma_1 \land \cdots \land \sigma_k) \rightarrow \tau) \equiv (\sigma_1 \implies (\sigma_2 \implies ( \cdots (\sigma_k \implies \tau))))\]


\section*{Exercise 7}
\begin{framed}
    Prove or refute each of the following assertions:
    \begin{enumerate}
        \item If either $\Sigma \models \alpha$ or $\Sigma \models \beta$, then $\Sigma \models (\alpha \lor \beta)$.
        \item If $\Sigma \models (\alpha \lor \beta)$, then either $\Sigma \models \alpha$ or $\Sigma \models \beta$. 
    \end{enumerate}
\end{framed}

Taking $\Sigma = \{\sigma_1, \sigma_2, \cdots, \sigma_n\}$

\subsection*{Assertion 1}

\begin{center}
    \begin{tabular}{r l l}
        1 & $((\sigma_1 \land \sigma_2 \land \cdots \land \sigma_n) \implies \alpha) \lor ((\sigma_1 \land \sigma_2 \land \cdots \land \sigma_n) \implies \beta)$ & Hypothesis \\
        \hline
        2 & $(\lnot(\sigma_1 \land \sigma_2 \land \cdots \land \sigma_n) \lor \alpha) \lor (\lnot(\sigma_1 \land \sigma_2 \land \cdots \land \sigma_n) \lor \beta)$ & Definition of Implication on line 1\\
        3 & $\lnot(\sigma_1 \land \sigma_2 \land \cdots \land \sigma_n) \lor (\alpha \lor \beta)$ & Distribution on line 2 \\
        \hline
        4 & $(\sigma_1 \land \sigma_2 \land \cdots \land \sigma_n) \implies (\alpha \lor \beta)$ & Definition of Implication on line 3
    \end{tabular}    
\end{center}

Therefore if $\Sigma \models \alpha$ or $\Sigma \models \beta$, then $\Sigma \vDash (\alpha \lor \beta)$.

\subsection*{Assertion 2}

\begin{center}
    \begin{tabular}{r l l}
        1 & $(\sigma_1 \land \sigma_2 \land \cdots \land \sigma_n) \implies (\alpha \lor \beta)$ & Hypothesis \\
        \hline
        2 & $\lnot(\sigma_1 \land \sigma_2 \land \cdots \land \sigma_n) \lor (\alpha \lor \beta)$ & Definition of Implication on line 1 \\
        3 & $(\lnot(\sigma_1 \land \sigma_2 \land \cdots \land \sigma_n) \lor \alpha) \lor (\lnot(\sigma_1 \land \sigma_2 \land \cdots \land \sigma_n) \lor \beta)$ & Distribution on line 2\\
        \hline
        4 & $((\sigma_1 \land \sigma_2 \land \cdots \land \sigma_n) \implies \alpha) \lor ((\sigma_1 \land \sigma_2 \land \cdots \land \sigma_n) \implies \beta)$ & Definition of Implication on line 3
    \end{tabular}    
\end{center}

Therefore if $\Sigma \vDash (\alpha \lor \beta)$, then $\Sigma \models \alpha$ or $\Sigma \models \beta$.


\section*{Exercise 8}
\begin{framed}
    Let $\Sigma$ and $\tau$ be, respectively, a set of wffs and a wff. Show that, if 
    $$\Sigma \cup \{\neg \tau\} \vdash F,$$
    then 
    $$\Sigma \vdash \tau.$$
\end{framed}

If we say $\Sigma = \{\sigma_1, \sigma_2, \cdots, \sigma_n\}$, then $\Sigma \cup \{\lnot \tau\} = \{\sigma_1, \sigma_2, \cdots, \sigma_n, \lnot \tau\}$. So

\begin{center}
    \begin{tabular}{r l l}
        1 & $((\sigma_1 \land \sigma_2 \land \cdots \land \sigma_n \land \lnot \tau) \implies F)$ & Hypothesis \\
        \hline
        2 & $(\lnot (\sigma_1 \land \sigma_2 \land \cdots \land \sigma_n \land \lnot \tau) \lor F)$ & Definition of Implication on line 1 \\
        3 & $\lnot (\sigma_1 \land \sigma_2 \land \cdots \land \sigma_n \land \lnot \tau)$ & Identity on line 2 \\
        4 & $(\lnot \sigma_1 \lor \lnot \sigma_2 \lor \cdots \lor \lnot \sigma_n \lor \tau)$ & De Morgan's Laws on line 3 \\
        5 & $(\lnot \sigma_1 \lor \lnot \sigma_2 \lor \cdots \lor \lnot \sigma_n) \lor \tau$ & Associativity of Disjunction on line 4 \\
        6 & $\lnot(\sigma_1 \land \sigma_2 \land \cdots \land \sigma_n) \lor \tau$ & De Morgan's Laws on line 5 \\
        \hline
        7 & $(\sigma_1 \land \sigma_2 \land \cdots \land \sigma_n) \implies \tau$ & Definition of Implication on line 6 
    \end{tabular}    
\end{center}

Therefore if $\Sigma \cup \{\lnot \tau\} \vdash F$, then $\Sigma \vdash \tau$.





\end{document}

